\documentclass{article}
\usepackage[english]{babel}
\usepackage{amsmath}
\usepackage{amssymb}
\usepackage{changepage}
\usepackage{amsthm}
\usepackage[margin=1in]{geometry}
\usepackage{fancyhdr}

\pagestyle{fancy}
\rhead{Stephen Nusko 103693282 \\ 60-231 Assignment 2}

\title{[03-60-231] Assignment 2}
\author{Stephen Nusko \\ 103693282}

\begin{document}
	\thispagestyle{empty}
	\maketitle	
	\section{Question 2.1}
		\subsection{Part c}
			Evaluate $(\forall x)(\exists y)(P(x) \Rightarrow Q(x, y))$ \\
			Let x = 1. We obtain $(\exists y)(P(1) \Rightarrow Q(1, y))$ \\
			Let y = 2. Then $P(1) \equiv T$ and $Q(1, 2) \equiv T$ \\
			Therefore $(\exists y)(P(1) \Rightarrow Q(1, y)$ is evaluated to true. \\
			Let x = 2. We obtain $(\exists y)(P(2) \Rightarrow Q(2, y)$ \\
			Since $P(2) \equiv F$ \\
			$\therefore (\exists y)(P(2) \Rightarrow Q(2, y))$ is evaluated to true. \\
			$\therefore (\forall x)(\exists y)(P(x) \Rightarrow Q(x, y))$ is evaluated to true. \\
		\subsection{Part i}
			Evaluate $(\exists x)(\exists y)(Q(x, a) \Rightarrow Q(b, y)$ \\
			Let x = 1. We obtain $(\exists y)(Q(1, a) \Rightarrow Q(b, y)$ \\
			Let y = 2. We obtarin $(Q(1, a) \Rightarrow Q(b, 2)$ \\
			since $Q(1, a) \equiv Q(1, 2) \equiv T \equiv Q(b, 2) \equiv Q(1, 2)$ \\
			$\therefore Q(1, 2) \Rightarrow Q(1, 2)$ is evaluated to true. \\
			$\therefore (\exists y)(Q(1, a) \Rightarrow Q(b, y))$ is evaluated to true. \\
			$\therefore (\exists x)(\exists y)(Q(x, a) \Rightarrow Q(b, y))$ is evaluated to true. \\
	\section{Question 2.2}
		\subsection{Part c}
			Prove $((\forall x)\alpha(x) \lor (\forall x)\beta(x)) \Rightarrow (\forall x)(\alpha(x) \lor \beta(x))$ \\
			Solution: (indirect proof) \\
			\begin{enumerate}
				\item $\lnot((\forall x)(\alpha(x) \lor \beta(x))$ \hfill Hypothesis
				\item $(\exists x)\lnot(\alpha(x) \lor \beta(x))$ \hfill 1, FE7
				\item $(\exists x)(\lnot\alpha(x) \land \lnot\beta(x))$ \hfill 2, E17
				\item $\lnot\alpha(c) \land \lnot\beta(c)$ \hfill 3, EI, c is a constant
				\item $\lnot\alpha(c)$ \hfill 4, I2 
				\item $\lnot\beta(c) \land \lnot\alpha(c)$ \hfill 4, E9 
				\item $\lnot\beta(c)$ \hfill 6, I2
				\item $(\exists x)\lnot\alpha(x)$ \hfill 5, EQ
				\item $(\exists x)\lnot\beta(x)$ \hfill 7, EQ
				\item $(\exists x)\lnot\alpha(x) \land (\exists x)\lnot\beta(x)$ \hfill 8, 9, I6
				\item $\lnot(\forall x)\alpha(x) \land (\exists x)\lnot\beta(x)$ \hfill 10, FE7
				\item $\lnot(\forall x)\alpha(x) \land \lnot(\forall x)\beta(x)$ \hfill 11, FE7
				\item $\lnot((\forall x)\alpha(x) \lor (\forall x)\beta(x))$ \hfill 12, E17
			\end{enumerate}
			$\therefore \lnot((\forall x)(\alpha(x) \lor \beta(x)) \Rightarrow \lnot((\forall x)\alpha(x) \lor (\forall x)\beta(x))$ \\
			$\therefore ((\forall x)\alpha(x) \lor (\forall x)\beta(x)) \Rightarrow (\forall x)(\alpha(x) \lor \beta(x))$ \hfill $\qed$ \\
		\subsection{Part d}
			Prove $(\forall x)(\alpha(x) \Rightarrow \beta(x)) \Rightarrow ((\forall x)\lnot\beta(x) \Rightarrow (\forall x)\lnot\alpha(x))$ \\
			Solution: (indirect proof) \\
			\begin{enumerate}
				\item $\lnot((\forall x)\lnot\beta(x) \Rightarrow (\forall x)\lnot\alpha(x))$ \hfill Hypothesis
				\item $\lnot(\lnot((\forall x)\lnot\beta(x)) \lor (\forall x)\lnot\alpha(x))$ \hfill 1, E18
				\item $\lnot\lnot(\forall x)\lnot\beta(x) \land \lnot(\forall x)\lnot\alpha(x))$ \hfill 2, E17
				\item $(\forall x)\lnot\beta(x) \land \lnot(\forall x)\lnot\alpha(x)$ \hfill 3, E15
				\item $(\forall x)\lnot\beta(x)$ \hfill 4, I2
				\item $\lnot(\forall x)\lnot\alpha(x) \land (\forall x)\lnot\beta(x)$ \hfill 4, E9
				\item $\lnot(\forall x)\lnot\alpha(x)$ \hfill 7, I2
				\item $(\exists x)\lnot\lnot\alpha(x)$ \hfill 8, FE7
				\item $\lnot\lnot\alpha(c)$ \hfill 8, EI
				\item $\lnot\beta(c)$ \hfill 5, UI 
				\item $\lnot\lnot\alpha(c) \land \lnot\beta(c)$ \hfill 9, 10, I6
				\item $(\exists x)(\lnot\lnot\alpha(x) \land \lnot\beta(x))$ \hfill 11, EQ
				\item $(\exists x)\lnot(\lnot\alpha(x) \lor \beta(x))$ \hfill 12, E17
				\item $\lnot((\forall x)(\lnot\alpha(x) \lor \beta(x)))$ \hfill 13, FE7
				\item $\lnot((\forall x)(\alpha(x) \Rightarrow \beta(x)))$ \hfill 14, E18
			\end{enumerate}
			$\therefore \lnot((\forall x)\lnot\beta(x) \Rightarrow (\forall x)\lnot\alpha(x)) \Rightarrow \lnot((\forall x)(\alpha(x) \Rightarrow \beta(x)))$ \\
			$\therefore (\forall x)(\alpha(x) \Rightarrow \beta(x)) \Rightarrow (\forall x)\lnot\beta(x) \Rightarrow (\forall x)\lnot\alpha(x)$ \hfill \qed \\
	\section{Question 2.3}
		\subsection{Part d}
			\begin{tabular}{r l}
				P1: & $(\exists x)(P(x) \land (\forall y)((R(y) \land S(x, y)) \Rightarrow Z(x, y))$ \\
				P2: & $(\forall x)(P(x) \Rightarrow (\exists y)(R(y) \land \lnot U(x, y) \land T(x, y))$ \\
				P3: & $(\forall x)(\forall y)((P(x) \land R(y) \land T(x, y)) \Rightarrow S(x, y)$ \\ \hline
				C: & $(\exists x)(\exists y)(P(x) \land R(x) \land Z(x, y) \land \lnot U(x, y))$ \\
			\end{tabular}
			\newline \\
			Prove: $((P1 \land P2 \land P3) \Rightarrow C)$ \\
			Solution: (direct proof) \\
			\begin{enumerate}
				\item $(\exists x)(P(x) \land (\forall y)((R(y) \land S(x, y)) \Rightarrow Z(x, y)))$ \hfill Hypothesis from P1
				\item $(\forall x)(P(x) \Rightarrow (\exists y)(R(y) \land \lnot U(x, y) \land T(x, y)))$ \hfill Hypothesis from P2
				\item $(\forall x)(\forall y)((P(x) \land R(y) \land T(x, y)) \Rightarrow S(x, y))$ \hfill Hypothesis from P3
				\item $P(c) \land (\forall y)((R(y) \land S(c, y)) \Rightarrow Z(c, y)$ \hfill 1, EI, c is a constant
				\item $P(c)$ \hfill 4, I2
				\item $(\exists y)(R(y) \land \lnot U(c, y) \land T(c, y)$ \hfill 5, 2, I3
				\item $R(k) \land \lnot U(c, k) \land T(c, k)$ \hfill 6, EI, k is a constant
				\item $R(k) \land \lnot U(c, k)$ \hfill 7, I2
				\item $R(k)$ \hfill 8, I2
				\item $\lnot U(c, k) \land R(k)$ \hfill 9, E9
				\item $\lnot U(c, k)$ \hfill 10, I2
				\item $T(c, k) \land R(k) \land \lnot U(c, k)$ \hfill 7, E9
				\item $T(c, k)$ \hfill 12, I2
				\item $P(c) \land R(k)$ \hfill 5, 9, I6
				\item $P(c) \land R(k) \land T(c, k)$ \hfill 14, 13, I6
				\item $S(c, k)$ \hfill 15, 3, I3
				\item $(\forall y)((R(y) \land S(c, y) \Rightarrow Z(c, y) \land P(c)$ \hfill 4, E9
				\item $(\forall y)((R(y) \land S(c, y) \Rightarrow Z(c, y)$ \hfill 17, I2
				\item $R(k) \land S(c, y)$ \hfill 9, 16, I6
				\item $Z(c, k)$ \hfill 19, 18, I3
				\item $P(c) \land R(k) \land Z(c, k)$ \hfill 14, 20, I6
				\item $P(c) \land R(k) \land Z(c, k) \land \lnot U(c, k)$ \hfill 21, 11, I6
				\item $(\exists y)(P(c) \land R(y) \land Z(c, y) \land \lnot U(c, y)$ \hfill 22, EQ
				\item $(\exists x)(\exists y)(P(x) \land R(y) \land Z(x, y) \land \lnot U(x, y)$ \hfill 23, EQ
			\end{enumerate}
			$\therefore ((P1 \land P2 \land P3) \Rightarrow C)$ \hfill $\qed$ \\
	\section{Question 2.4}
		\subsection{Part f}
		The universe of discourse are poems. \\
			Let I(x) denote an interesting poem. \\
			Let M(x) denote a modern poem. \\
			Let F(x) denote a poem written by me. \\
			Let S(x) denote a poem written about a soap bubble. \\
			Let R(x) denote a poem that is popular with people of real taste. \\
			Let A(x) denote a poem that is affected. \\
			\newline
			\begin{tabular}{r l}
				P1: & $\lnot(\exists x)(I(x) \land \lnot R(x))$ \\
				P2: & $\lnot(\exists x)(M(x) \land \lnot B(x))$ \\
				P3: & $(\forall x)(F(x) \Rightarrow S(x))$ \\
				P4: & $\lnot(\exists x)(B(x) \land R(x))$ \\
				P5: & $\lnot(\exists x)(\lnot M(x) \land S(x))$ \\ \hline
				C: & $(\forall x)(F(x) \Rightarrow \lnot I(x))$ \\
			\end{tabular}
			\newline \\
			Prove $((P1 \land P2 \land P3 \land P4 \land P5) \Rightarrow C)$ \\
			Solution: (direct proof)
			\begin{enumerate}
				\item $\lnot(\exists x)(I(x) \land \lnot R(x))$ \hfill Hypothesis from P1
				\item $\lnot(\exists x)(M(x) \land \lnot B(x))$ \hfill Hypothesis from P2
				\item $(\forall x)(F(x) \Rightarrow S(x))$ \hfill Hypothesis from P3
				\item $\lnot(\exists x)(B(x) \land R(x))$ \hfill Hypothesis from P4
				\item $\lnot(\exists x)(\lnot M(x) \land S(x))$ \hfill Hypothesis from P5
				\item $(\forall x)\lnot(I(x) \land \lnot R(x))$ \hfill 1, FE8
				\item $(\forall x)(\lnot I(x) \lor \lnot\lnot R(x))$ \hfill 6, E16
				\item $(\forall x)(\lnot\lnot R(x) \lor \lnot I(x))$ \hfill 7, E10
				\item $(\forall x)(\lnot R(x) \Rightarrow \lnot I(x))$ \hfill 8, E18
				\item $\lnot R(x) \Rightarrow \lnot I(x)$ \hfill 9, UI
				\item $(\forall x)\lnot(\lnot M(x) \land S(x))$ \hfill 5, FE8
				\item $(\forall x)(\lnot\lnot M(x) \lor \lnot S(x))$ \hfill 11, E16
				\item $(\forall x)(\lnot S(x) \lor \lnot\lnot M(x))$ \hfill 12, E10
				\item $(\forall x)(\lnot S(x) \lor M(x))$ \hfill 13, E15
				\item $(\forall x)(S(x) \Rightarrow M(x))$ \hfill 14, E18
				\item $S(x) \Rightarrow M(x)$ \hfill 15, UI
				\item $(\forall x)\lnot(M(x) \land \lnot B(x))$ \hfill 2, FE8
				\item $(\forall x)(\lnot M(x) \lor \lnot\lnot B(x))$ \hfill 17, E16
				\item $(\forall x)(\lnot M(x) \lor B(x))$ \hfill 18, E15
				\item $(\forall x)(M(x) \Rightarrow B(x))$ \hfill 19, E18
				\item $M(x) \Rightarrow B(x)$ \hfill 20, UI
				\item $(\forall x)\lnot(B(x) \land R(x))$ \hfill 4, FE8
				\item $(\forall x)(\lnot B(x) \lor \lnot R(x))$ \hfill 22, E16
				\item $(\forall x)(B(x) \Rightarrow \lnot R(x))$ \hfill 23, E18
				\item $B(x) \Rightarrow \lnot R(x)$ \hfill 24, UI
				\item $S(x) \Rightarrow B(x)$ \hfill 16, 21, I5
				\item $S(x) \Rightarrow \lnot R(x)$ \hfill 26, 25, I5
				\item $S(x) \Rightarrow \lnot I(x)$ \hfill 27, 10, I5
				\item $F(x) \Rightarrow \lnot I(x)$ \hfill 3, 28, I5
			\end{enumerate}
			$\therefore ((P1 \land P2 \land P3 \land P4 \land P5) \Rightarrow C)$ \hfill $\qed$ \\
\end{document}
